Test/Reduction.lean
@@ -1,4 +1,5 @@
 import Auto.Lib.ExprExtra
+import Auto.Lib.BinTree
 
 set_option lazyReduce.printTime true
 set_option maxRecDepth 50000 in
@@ -25,3 +26,33 @@ def tst1₁ (x : α) : True :=
   let a := inferInstanceAs (Inhabited Nat);
   let b := a.default
   True.intro
+
+open Auto
+
+def simplebt (x : Nat) (n : Nat) : BinTree Nat :=
+  match n with
+  | 0 => .leaf
+  | n' + 1 => .node (simplebt (2 * x) n') (.some x) (simplebt (2 * x + 1) n')
+
+def foldl' (f : α → β → α) (init : α) : BinTree β → α
+| .leaf => init
+| .node l x r =>
+  let lf := foldl' f init l
+  let mf :=
+    match x with
+    | .some x => f lf x
+    | .none => lf
+  match mf with
+  | mf => foldl' f mf r
+
+def foldAgain (bt : BinTree Nat) := foldl' (fun bt entry => bt.insert entry entry) BinTree.leaf bt
+
+/-
+def sdk : (foldAgain (simplebt 1 12)).get? 100 = Option.some 100 := Eq.refl (Option.some 100)
+
+#check (simplebt 2 10)
+
+#eval (foldAgain (simplebt 1 12)).get? 100
+-/
+
+#check 2
